Still have to figure out names

.Makefile.d
@@ -1,9 +1,9 @@
 theories/AsmGen.vo theories/AsmGen.glob theories/AsmGen.v.beautified theories/AsmGen.required_vo: theories/AsmGen.v theories/CpdtTactics.vo
 theories/AsmGen.vio: theories/AsmGen.v theories/CpdtTactics.vio
 theories/AsmGen.vos theories/AsmGen.vok theories/AsmGen.required_vos: theories/AsmGen.v theories/CpdtTactics.vos
-theories/progLog.vo theories/progLog.glob theories/progLog.v.beautified theories/progLog.required_vo: theories/progLog.v theories/AsmGen.vo
-theories/progLog.vio: theories/progLog.v theories/AsmGen.vio
-theories/progLog.vos theories/progLog.vok theories/progLog.required_vos: theories/progLog.v theories/AsmGen.vos
+theories/progLog.vo theories/progLog.glob theories/progLog.v.beautified theories/progLog.required_vo: theories/progLog.v theories/CpdtTactics.vo theories/AsmGen.vo
+theories/progLog.vio: theories/progLog.v theories/CpdtTactics.vio theories/AsmGen.vio
+theories/progLog.vos theories/progLog.vok theories/progLog.required_vos: theories/progLog.v theories/CpdtTactics.vos theories/AsmGen.vos
 theories/CpdtTactics.vo theories/CpdtTactics.glob theories/CpdtTactics.v.beautified theories/CpdtTactics.required_vo: theories/CpdtTactics.v 
 theories/CpdtTactics.vio: theories/CpdtTactics.v 
 theories/CpdtTactics.vos theories/CpdtTactics.vok theories/CpdtTactics.required_vos: theories/CpdtTactics.v 
