theories/progLog2.v
@@ -1,0 +1,31 @@
+From iris.proofmode Require Import proofmode.
+From iris.base_logic Require Export invariants gen_heap.
+From iris.program_logic Require Export weakestpre ectx_lifting.
+From iris.algebra Require Import frac auth gmap excl.
+From Coq.Lists Require Import List.
+From ASMinCoq Require Import CpdtTactics.
+From ASMinCoq Require Import AsmGen progLog.
+
+
+
+
+(* invariants for memory, and a state interpretation for (mem,reg) *)
+Global Instance memG_irisG `{!invG Σ, !memG Σ, !regG Σ, !traceG (list leak) Σ, !pcG Σ, !programG Σ,
+    !memG Σ', !regG Σ', !traceG (list leak) Σ', !pcG Σ', !programG Σ'} :
+      irisGS asm_lang2 (Σ * Σ')
+      := {
+  iris_invGS := inv_invG;
+  state_interp σ _ κs _ :=
+    ((gen_heap_interp (reg σ.1.1.2)) ∗
+    (gen_heap_interp (mem σ.1.1.2)) ∗
+    tr_auth trace_name σ.2 ∗ pc_auth PC_name (PC σ.1.1.2) ∗
+    program_auth Program_name σ.1.1.1
+    ∗
+    (gen_heap_interp (reg σ.2.1.2)) ∗
+    (gen_heap_interp (mem σ.2.1.2)) ∗
+    tr_auth trace_name σ.2.2 ∗ pc_auth PC_name (PC σ.2.1.2) ∗
+    program_auth Program_name σ.2.1.1)%I;
+  fork_post _ := False%I;
+  num_laters_per_step _ := 0;
+  state_interp_mono _ _ _ _ := fupd_intro _ _
+}.
